Add soundness definitions for different datatypes
There are now definitions for the soundness of parity, abstract
booleans, states, commands and expressions.

AbstractBool.v
@@ -33,21 +33,31 @@ Definition extract_bool (b: bool) : abstr_bool :=
   | false => ab_false
   end.
 
+Definition sound_ab (ab: abstr_bool) (b: bool) := gamma_bool ab b.
+
 (** * Operations *)
 
 (** ** And *)
 
 Definition and_ab (b1 b2 : abstr_bool) : abstr_bool :=
-  match b1, b2 with
-  | ab_bottom, _         => ab_bottom
-  | _        , ab_bottom => ab_bottom
-  | ab_false , _         => ab_false
-  | _        , ab_false  => ab_false
-  | ab_top   , ab_true   => ab_top
-  | ab_true  , ab_top    => ab_top
-  | ab_top   , ab_top    => ab_top
-  | ab_true  , ab_true   => ab_true
+  match b1 with
+  | ab_bottom => ab_bottom
+  | ab_true   => b2
+  | ab_top    => match b2 with
+                 | ab_bottom => ab_bottom
+                 | ab_false  => ab_false
+                 | _         => ab_top
+                 end
+  | ab_false  => match b2 with
+                 | ab_bottom => ab_bottom
+                 | _ => ab_false
+                 end
   end.
+
+Example and_ab1 : and_ab ab_bottom ab_top = ab_bottom. reflexivity. Qed.
+Example and_ab2 : and_ab ab_true ab_true = ab_true. reflexivity. Qed.
+Example and_ab3 : and_ab ab_true ab_false = ab_false. reflexivity. Qed.
+Example and_ab4 : and_ab ab_top  ab_true = ab_top. reflexivity. Qed.
 
 Lemma and_ab_comm : forall b1 b2, and_ab b1 b2 = and_ab b2 b1.
 Proof. destruct b1, b2; reflexivity. Qed.
@@ -56,25 +66,33 @@ Lemma and_ab_assoc : forall b1 b2 b3,
   and_ab (and_ab b1 b2) b3 = and_ab b1 (and_ab b2 b3).
 Proof. destruct b1, b2, b3; reflexivity. Qed.
 
-Lemma and_ab_trans : forall b1 b2 b3,
-  and_ab b1 b2 = ab_true -> and_ab b2 b3 = ab_true -> and_ab b1 b3 = ab_true.
-Proof.
-  intros. destruct b1, b2, b3; try reflexivity; try inversion H0; try inversion
-  H.
+Lemma and_ab_sound : forall ab1 ab2 b1 b2,
+  sound_ab ab1 b1 ->
+  sound_ab ab2 b2 ->
+  sound_ab (and_ab ab1 ab2) (andb b1 b2).
+Proof. intros. destruct ab1; destruct b1; inversion H.
+  - simpl. assumption.
+  - destruct ab2; try inversion H0; try reflexivity.
+  - destruct ab2; try inversion H0; try reflexivity. 
+    simpl. destruct b2; try reflexivity; try inversion H0.
+  - destruct ab2; try reflexivity. inversion H0.
 Qed.
 
 (** ** Or *)
 
 Definition or_ab (b1 b2 : abstr_bool) : abstr_bool :=
-  match b1, b2 with
-  | ab_bottom, _ => ab_bottom
-  | _, ab_bottom => ab_bottom
-  | ab_true, _   => ab_true
-  | _ , ab_true  => ab_true
-  | ab_top, ab_false => ab_top
-  | ab_false, ab_top => ab_top
-  | ab_top, ab_top  => ab_top
-  | ab_false, ab_false => ab_false
+  match b1 with
+  | ab_bottom => ab_bottom
+  | ab_false  => b2
+  | ab_top    => match b2 with
+                 | ab_bottom => ab_bottom
+                 | ab_true   => ab_true
+                 | _         => ab_top
+                 end
+  | ab_true   => match b2 with
+                 | ab_bottom => ab_bottom
+                 | _         => ab_true
+                 end
   end.
 
 Lemma or_ab_comm : forall b1 b2, or_ab b1 b2 = or_ab b2 b1.
@@ -84,4 +102,16 @@ Lemma or_ab_assoc : forall b1 b2 b3,
   or_ab (or_ab b1 b2) b3 = or_ab b1 (or_ab b2 b3).
 Proof. intros. destruct b1, b2, b3; reflexivity. Qed.
 
+Lemma or_ab_sound : forall ab1 ab2 b1 b2,
+  sound_ab ab1 b1 ->
+  sound_ab ab2 b2 ->
+  sound_ab (or_ab ab1 ab2) (orb b1 b2).
+Proof. intros. destruct ab1; destruct b1; inversion H.
+  - destruct ab2; try reflexivity; try inversion H0.
+  - simpl. assumption.
+  - destruct ab2; try reflexivity; try inversion H0.
+  - destruct ab2; try reflexivity. 
+    + simpl. destruct b2; try reflexivity; try inversion H0.
+    + inversion H0.
+Qed.
 
