AbstractInterpreter.v
@@ -1,8 +1,8 @@
+Require Import AbstractState.
+Require Import ConcreteInterpreter.
 Require Import Language.
 Require Import Maps.
 Require Import Parity.
-
-Definition abstract_state := total_map parity.
 
 Open Scope com_scope.
 
@@ -16,6 +16,10 @@ Fixpoint abstract_eval_aexp (st : abstract_state) (e : aexp) : parity :=
       parity_mult (abstract_eval_aexp st p1) (abstract_eval_aexp st p2)
   end.
 
+Definition sound_aexp (e : aexp) := forall ast st,
+  sound_state ast st -> 
+  sound_par (abstract_eval_aexp ast e) (eval_aexp st e).
+
 Fixpoint ceval_abstract (st : abstract_state) (c : com) : abstract_state :=
   match c with
   | CSkip => st
@@ -25,4 +29,7 @@ Fixpoint ceval_abstract (st : abstract_state) (c : com) : abstract_state :=
   | x ::= a => t_update st x (abstract_eval_aexp st a)
   end.
 
+Definition sound_com (c : com) := forall ast st,
+  sound_state ast st -> 
+  sound_state (ceval_abstract ast c) (ceval st c).
 
