practice.v
@@ -10,67 +10,66 @@ Require Import Parity.
 Require Import Maps.
 Require Import Language.
 
-Definition state := total_map nat.
-
-Definition abstract_state := total_map (parity).
-
 Open Scope com_scope.
 
-Lemma abstract_aexp_plus_sound : forall st ast e1 e2,
-  gamma_par (abstract_eval_aexp ast e1) (eval_aexp st e1) ->
-  gamma_par (abstract_eval_aexp ast e2) (eval_aexp st e2) ->
-  gamma_par (abstract_eval_aexp ast (APlus e1 e2)) (eval_aexp st (APlus e1 e2)).
-Proof.
-  intros. simpl. apply gamma_distr_plus; assumption.
+Lemma abstract_aexp_plus_sound : forall e1 e2,
+  sound_aexp e1 ->
+  sound_aexp e2 ->
+  sound_aexp (APlus e1 e2).
+Proof. 
+  unfold sound_aexp. intros. simpl. apply parity_plus_sound. 
+  apply H. assumption.
+  apply H0. assumption.
 Qed.
 
-Lemma abstract_aexp_mult_sound : forall ast st e1 e2,
-  gamma_par (abstract_eval_aexp ast e1) (eval_aexp st e1) ->
-  gamma_par (abstract_eval_aexp ast e2) (eval_aexp st e2) ->
-  gamma_par (abstract_eval_aexp ast (AMult e1 e2)) (eval_aexp st (AMult e1 e2)).
-Proof. intros. simpl. apply gamma_distr_mult; assumption.
-Qed.
-
-Lemma abstract_aexp_var_sound : forall ast st x,
-  sound_state ast st ->
-  gamma_par (abstract_eval_aexp ast (AVar x)) (eval_aexp st (AVar x)).
-Proof. intros. simpl. auto. Qed.
-
-Theorem abstract_aexp_eval_sound : forall ast st e,
-  sound_state ast st ->
-  (gamma_par (abstract_eval_aexp ast e)) (eval_aexp st e).
+Lemma abstract_aexp_mult_sound : forall e1 e2,
+  sound_aexp e1 ->
+  sound_aexp e2 ->
+  sound_aexp (AMult e1 e2).
 Proof.
+  unfold sound_aexp. intros. apply parity_mult_sound. apply H. assumption.
+  apply H0. assumption. Qed.
+
+Lemma abstract_aexp_var_sound : forall x,
+  sound_aexp (AVar x).
+Proof. intros. unfold sound_aexp. intros. simpl. unfold sound_state in H.
+  apply H. Qed.
+
+
+Theorem abstract_aexp_eval_sound : forall e,
+  sound_aexp e.
+Proof. 
   induction e; intros.
-  - (* ANum *) simpl. apply gamma_extract_n_n.
-  - (* AVar *) apply abstract_aexp_var_sound. apply H.
-
+  - (* ANum *) unfold sound_aexp. intros. simpl. apply gamma_extract_n_n.
+  - (* AVar *) apply abstract_aexp_var_sound. 
   - (* APlus *) apply abstract_aexp_plus_sound; auto.
   - (* AMult *) apply abstract_aexp_mult_sound; auto.
 Qed.
 
-Lemma abstract_ceval_ass_sound : forall ast st y a,
-  sound_state ast st ->
-  sound_state (ceval_abstract ast (y ::= a)) (ceval st (y ::= a)).
+Lemma abstract_ceval_ass_sound : forall y a,
+  sound_com (y ::= a).
 Proof.
+  unfold sound_com. 
   intros. simpl. unfold t_update, sound_state. intros.
   destruct (beq_string y x). 
   - apply abstract_aexp_eval_sound. apply H.
   - unfold sound_state in H. apply H.
 Qed.
 
-Theorem abstract_ceval_sound : forall ast st c,
-  sound_state ast st ->
-  sound_state (ceval_abstract ast c) (ceval st c).
-Proof.
-  unfold sound_state. intros ast st c. revert ast st.
-  induction c.
-  - (* SKIP *) auto.
-  - (* CSeq *) simpl. intros.
-    apply IHc2. clear IHc2. intros. apply IHc1. apply H.
-  - intros. apply abstract_ceval_ass_sound. unfold sound_state. apply H.
+Lemma abstract_ceval_seq_sound : forall c1 c2,
+  sound_com c1 ->
+  sound_com c2 ->
+  sound_com (c1 ;; c2).
+Proof. 
+  unfold sound_com. intros. apply H0. apply H. assumption.
 Qed.
 
-(* Add a statements SKIP, sequencing, if statements, assignment *)
+Theorem abstract_ceval_sound : forall c,
+  sound_com c.
+Proof. 
+  intros c. induction c; intros.
+  - (* SKIP *) unfold sound_com. simpl. intros. assumption.
+  - (* CSeq *) apply abstract_ceval_seq_sound; assumption.
+  - apply abstract_ceval_ass_sound.
+Qed.
 
-(* TODO abstract store *)
-(* TODO abstract bool *)
