AbstractState.v
@@ -6,3 +6,14 @@ Definition abstract_state := total_map parity.
 
 Definition sound_state (ast : abstract_state) (st : state) : Prop := 
   forall x, gamma_par (ast x) (st x).
+
+Lemma t_update_sound : forall ast st x p n,
+  sound_state ast st ->
+  sound_par p n ->
+  sound_state (t_update ast x p) (t_update st x n).
+Proof. 
+  intros. unfold sound_state.  intros. unfold t_update. 
+  destruct (beq_string x x0). 
+  - unfold sound_par in H0. assumption.
+  - unfold sound_state in H. apply H.
+Qed.
